forloop
git-svn-id: svn://scm.gforge.inria.fr/svn/cfml@176 ba02c806-7d2b-4818-9a48-35b22e6bdc79

imper/Loops.ml
@@ -1,0 +1,12 @@
+
+(* todo: why body has type int->'a without annotation?*)
+
+let loop_for a b (body:int->unit) =
+   let rec aux i =
+      if i <= b then (body i; aux (i+1)) in
+   aux a
+
+let loop_while cond (body:unit->unit) =
+   let rec aux () =
+      if cond() then (body(); aux()) in
+   aux()
