CFSpec.v
@@ -750,8 +750,141 @@ Qed.
 
 End SpecWeaken.
 
+
 (********************************************************************)
 (* ** Induction lemmas for spec *)
+
+Lemma spec_induction_1_noheap : 
+  forall A1 B,
+  forall (lt:binary A1) (Wf: wf lt) f (K:A1->~~B->Prop),
+  spec_1 (fun x R => 
+    spec_1 (fun x' R' => lt x' x -> K x' R') f ->
+    K x R) f ->
+  spec_1 K f.
+Proof.
+  introv W H.
+  cuts Hyp: (forall x, is_spec_0 (K x) /\ K x (app_1 f x)).
+    apply spec_intro_1. 
+      intros x. apply (proj1 (Hyp x)).
+      apply* spec_curried_1.
+      intros x. destruct~ (Hyp x). 
+  intros x. pattern x. induction_wf IH: W x.
+  lets C: (spec_curried_1 H). 
+  lets I: (proj1 H x).
+  lets S: (spec_elim_1 H x). clear H. 
+  asserts M: (spec_1 (fun x' R' => lt x' x -> K x' R') f). split.
+    intros x'. introv HK HP Lt. applys~ (proj1 (IH _ Lt)).
+    intros x' Lt. apply (proj2 (IH _ Lt)).
+  split.
+    introv HK HP. applys~ (I R R').
+    apply~ S.
+Qed.
+
+
+Lemma spec_induction_1 : 
+  forall A1 B A0,
+  forall (lt:binary (A0*A1)) (Wf: wf lt) f (L:A0->A1->~~B->Prop),
+  (forall y, is_spec_1 (L y)) ->
+  spec_1 (fun x R => forall y,
+    spec_1 (fun x' R' => forall y', lt (y',x') (y,x) -> L y' x' R') f ->
+    L y x R) f ->
+  spec_1 (fun x R => forall y, L y x R) f.
+Proof.
+  introv W Is H. 
+  cuts Hyp: (forall y x, is_spec_0 (L y x) /\ L y x (app_1 f x)).
+    apply spec_intro_1.
+      intros x. introv HK HP. intros y. applys~ (proj1 (Hyp y x)).
+      apply* spec_curried_1.
+      intros y x. destruct~ (Hyp x y).
+  cuts Hyp': (forall p, let '(y,x) := p in is_spec_0 (L y x) /\ L y x (app_1 f x)).
+    intros y x. apply (Hyp' (y,x)).
+  intros p. induction_wf IH: W p. destruct p as [y x].
+  lets C: (spec_curried_1 H). 
+  lets I: (proj1 H x).
+  lets S: (spec_elim_1 H x y). clear H.
+  split.
+    apply~ Is.
+    apply S. split.
+      intros x'. introv HK HP Lt. applys~ (proj1 (IH _ Lt)).
+      intros x' y' Lt. apply (proj2 (IH _ Lt)).
+Qed.
+
+Lemma spec_induction_1_noarg : 
+  forall A1 B A0,
+  forall (lt:binary A0) (Wf: wf lt) f (L:A0->A1->~~B->Prop),
+  (forall y, is_spec_1 (L y)) ->
+  spec_1 (fun x R => forall y,
+    spec_1 (fun x' R' => forall y', lt y' y -> L y' x' R') f ->
+    L y x R) f ->
+  spec_1 (fun x R => forall y, L y x R) f.
+Proof.
+  introv W Is H. applys* spec_induction_1 (unproj21_wf (A2:=A1) W).
+Qed. 
+
+
+Axiom spec_induction_2 : 
+  forall A1 A2 B A0 (lt:(A0*A1*A2)->(A0*A1*A2)->Prop),
+  forall (Wf: wf lt) f (L:A0->A1->A2->~~B->Prop),
+  (forall y, is_spec_2 (L y)) ->
+  spec_2 (fun x1 x2 R => forall x0,
+    spec_2 (fun y1 y2 R' => forall y0, lt (y0,y1,y2) (x0,x1,x2) -> L y0 y1 y2 R') f ->
+    L x0 x1 x2 R) f ->
+  spec_2 (fun x1 x2 R => forall x0, L x0 x1 x2 R) f.
+
+(* todo: monter les ordres *)
+Axiom spec_induction_3 :
+  forall A1 B A0,
+  forall (lt:binary (A0*A1)) (Wf: wf lt) f (L:A0->A1->~~B->Prop),
+  (forall y, is_spec_1 (L y)) ->
+  spec_1 (fun x R => forall y,
+    spec_1 (fun x' R' => forall y', lt (y',x') (y,x) -> L y' x' R') f ->
+    L y x R) f ->
+  spec_1 (fun x R => forall y, L y x R) f.
+Axiom spec_induction_4 : 
+  forall A1 B A0,
+  forall (lt:binary (A0*A1)) (Wf: wf lt) f (L:A0->A1->~~B->Prop),
+  (forall y, is_spec_1 (L y)) ->
+  spec_1 (fun x R => forall y,
+    spec_1 (fun x' R' => forall y', lt (y',x') (y,x) -> L y' x' R') f ->
+    L y x R) f ->
+  spec_1 (fun x R => forall y, L y x R) f.
+
+
+(*
+
+Definition with_pre (H:hprop) B (R:~~B) :=
+  fun (H':hprop) (Q:B->hprop) => H = H' /\ R H Q.
+
+Lemma spec_induction_1 : 
+  forall A1 B A' (I:A'->hprop),
+  forall (lt:binary (A1*A')) (Wf: wf lt) f (K:A1->~~B->Prop),
+  spec_1 (fun x R => forall y,
+    spec_1 (fun x' R' => forall y', lt (x',y') (x,y) -> K x' (with_pre (I y') R')) f ->
+    K x (with_pre (I y) R)) f ->
+  spec_1 K f.
+Proof.
+  introv W H.
+  cuts Hyp: (forall x, is_spec_0 (K x) /\ K x (app_1 f x)).
+    apply spec_intro_1. 
+      intros x. apply (proj1 (Hyp x)).
+      apply* spec_curried_1.
+      intros x. destruct~ (Hyp x).
+  cuts Hyp': (forall x y, is_spec_0 (K x) /\ K x (with_pre (I y) (app_1 f x))).
+    
+  intros x. pattern x.   induction_wf IH: W x.
+  lets C: (spec_curried_1 H). 
+  lets I: (spec_is_spec_1 H x).
+  lets S: (spec_elim_1 H x). clear H. 
+  asserts M: (spec_1 (fun x' R' => lt x' x -> K x' R') f). split.
+    intros x'. introv HK HP Lt. applys~ (proj1 (IH _ Lt)).
+    intros x' Lt. apply (proj2 (IH _ Lt)).
+  split.
+    introv HK HP. applys~ (I P P').
+    apply~ S.
+Qed.
+
+
+
 
 Definition post_for (h:heap) B (R:~~B) :=
   fun (H:hprop) (Q:B->hprop) => H h -> R H Q.
@@ -764,7 +897,7 @@ Lemma spec_induction_1 :
     K x (post_for h R)) f ->
   spec_1 K f.
 Admitted.
-(*
+
 Proof.
   introv W H.
   cuts I: (forall x, weakenable (K x) /\ K x (app_1 f x)).
