imper/Loops_proof.v
@@ -1,0 +1,56 @@
+Set Implicit Arguments.
+Require Import CFPrim Loops_ml.
+
+
+(********************************************************************)
+(* ** For loops *)
+
+Lemma loop_for_spec : 
+  Spec loop_for a b body |R>>
+       (a > (b)%Z -> R [] (#[])) 
+    /\ (a <= (b)%Z -> forall I,
+          (Spec body i |R>> a <= i <= b -> R (I i) (# I(i+1))) ->
+          R (I a) (# I ((b)%Z+1))).
+Proof.
+  xcf. intros. split; intros Cmp. 
+  (* case a > b *)
+  xfun (fun f => Spec f i |R>> i > b -> R [] (#[])).
+    intros Gt. xif. math. xret. xsimpl.
+  xapp~. hsimpl.
+  (* case a <= b *)
+  intros I Hbody.
+  xfun_noxbody (fun f => Spec f i |R>> a <= i <= b+1 -> R (I i) (# I (b+1))).
+    apply (spec_induction_1_noheap (lt:=upto (b+1))). prove_wf.
+    xbody. intros IH Le. 
+    xif.
+      xapp. math.
+       xapp; auto with maths.
+      xret. math_rewrite (i = b+1). auto.
+  xapp. math. xsimpl.
+Qed.
+    
+
+(********************************************************************)
+(* ** While loops *)
+
+
+
+
+(*
+Notation "'For' i '=' a 'To' b 'Do' Q1 'Done'" :=
+  (!For (fun H Q => (a > (b)%Z -> H ==> (Q tt)) /\ (a <= (b)%Z -> exists H', exists I,
+       (H ==> I a \* H') 
+    /\ (forall i, a <= i /\ i <= (b)%Z -> Q1 (I i) (# I(i+1))) 
+    /\ (I ((b)%Z+1) \* H' ==> Q tt))))
+  (at level 69, i ident) : charac.
+
+Notation "'While' Q1 'Do' Q2 'Done'" :=
+  (!While (fun H Q => exists H', exists A, exists I, exists R,
+       wf R 
+     /\ (exists x, H ==> I x \* H')
+     /\ (forall x, local (fun Hl Ql => exists Q', 
+            Q1 Hl Q'
+         /\ Q2 (Q' true) (# Hexists y, (I y) \* [R y x])
+         /\ (Q' false \* H' ==> Ql tt)) (I x) Q)))
+  (at level 69) : charac.
+*)
